theories/Operational/Awkernel/MinimalProjection.v
@@ -13,9 +13,11 @@ From RocqSched Require Import Operational.Common.OSAdapterContract.
 From RocqSched Require Import Operational.Common.OSCausalityContract.
 From RocqSched Require Import Operational.Common.OSSchedulerViewContract.
 From RocqSched Require Import Operational.Common.OSHandoffContract.
+From RocqSched Require Import Operational.Common.OSCandidateSourceContract.
 From RocqSched Require Import Refinement.OSCausalityTheorem.
 From RocqSched Require Import Refinement.OSSchedulerViewTheorem.
 From RocqSched Require Import Refinement.OSHandoffTheorem.
+From RocqSched Require Import Refinement.OSCandidateSourceTheorem.
 From RocqSched Require Import Refinement.OSRefinementTheorem.
 From RocqSched Require Import Operational.Common.ProjectionLemmas.
 From RocqSched Require Import Operational.Common.ProjectionInvariants.
@@ -84,6 +86,12 @@ Definition awk_labeled_concrete_scheduler_handoff_contract :=
 
 Definition awk_local_scheduler_handoff_contract :=
   @os_local_scheduler_handoff_contract AwkernelState.
+
+Definition awk_labeled_concrete_candidate_source_contract :=
+  @labeled_concrete_candidate_source_contract AwkernelState.
+
+Definition awk_local_candidate_source_adapter_contract :=
+  @os_local_candidate_source_adapter_contract AwkernelState.
 
 Definition awk_adapter_contract :=
   @os_multicore_adapter_contract AwkernelState.
