theories/Operational/Common/OSCandidateSourceContract.v
@@ -1,0 +1,99 @@
+From Stdlib Require Import List.
+Import ListNotations.
+From RocqSched Require Import Foundation.Base.
+From RocqSched Require Import Semantics.Schedule.
+From RocqSched Require Import Abstractions.SchedulingAlgorithm.SchedulerBridge.
+From RocqSched Require Import Multicore.Common.MultiCoreBase.
+From RocqSched Require Import Multicore.Common.Admissibility.
+From RocqSched Require Import Operational.Common.State.
+From RocqSched Require Import Operational.Common.OSProjectionInterface.
+From RocqSched Require Import Operational.Common.ConcreteExecution.
+From RocqSched Require Import Operational.Common.Projection.
+From RocqSched Require Import Operational.Common.OSLocalAdapterContract.
+From RocqSched Require Import Operational.Common.OSSchedulerViewContract.
+
+Definition projected_candidate_list
+    {CState : Type}
+    {P : OSLabeledProjection CState}
+    (jobs : JobId -> Job)
+    (m : nat)
+    (ex : labeled_concrete_execution P m)
+    (candidates_of : CandidateSource)
+    (t : Time) : list JobId :=
+  candidates_of
+    jobs
+    m
+    (project_schedule (osl_to_op_trace P (lce_trace ex)))
+    t.
+
+Record labeled_concrete_candidate_source_contract
+    {CState : Type}
+    {P : OSLabeledProjection CState}
+    (jobs : JobId -> Job)
+    (m : nat)
+    (candidates_of : CandidateSource)
+    (ex : labeled_concrete_execution P m) : Prop :=
+  mkLabeledConcreteCandidateSourceContract {
+    lccsc_candidates_visible :
+      forall t j,
+        In j (projected_candidate_list jobs m ex candidates_of t) ->
+        op_job_visible
+          m
+          (os_to_op_state (osl_to_os_projection P) (lce_trace ex t))
+          j;
+    lccsc_current_in_candidates :
+      forall t c j,
+        c < m ->
+        op_current
+          (os_to_op_state (osl_to_os_projection P) (lce_trace ex t))
+          c = Some j ->
+        In j (projected_candidate_list jobs m ex candidates_of t);
+    lccsc_runnable_in_candidates :
+      forall t j,
+        In j
+           (op_runnable
+              (os_to_op_state (osl_to_os_projection P) (lce_trace ex t))) ->
+        In j (projected_candidate_list jobs m ex candidates_of t);
+    lccsc_dispatch_target_in_candidates :
+      forall t c j,
+        c < m ->
+        op_dispatch_target
+          (os_to_op_state (osl_to_os_projection P) (lce_trace ex t))
+          c = Some j ->
+        In j (projected_candidate_list jobs m ex candidates_of t);
+    lccsc_prefix_extensional :
+      forall s1 s2 t,
+        (forall t' c, t' < t -> s1 t' c = s2 t' c) ->
+        candidates_of jobs m s1 t = candidates_of jobs m s2 t;
+  }.
+
+Arguments lccsc_candidates_visible
+  {CState P jobs m candidates_of ex} _ _ _ _.
+Arguments lccsc_current_in_candidates
+  {CState P jobs m candidates_of ex} _ _ _ _ _.
+Arguments lccsc_runnable_in_candidates
+  {CState P jobs m candidates_of ex} _ _ _ _.
+Arguments lccsc_dispatch_target_in_candidates
+  {CState P jobs m candidates_of ex} _ _ _ _ _.
+Arguments lccsc_prefix_extensional
+  {CState P jobs m candidates_of ex} _ _ _ _ _.
+
+Record os_local_candidate_source_adapter_contract
+    {CState : Type}
+    (P : OSLabeledProjection CState)
+    (candidates_of : CandidateSource)
+    (jobs : JobId -> Job)
+    (adm : admissible_cpu)
+    (m : nat) : Type :=
+  mkOSLocalCandidateSourceAdapterContract {
+    olcsac_base : os_local_multicore_adapter_contract P jobs adm m;
+    olcsac_candidates :
+      labeled_concrete_candidate_source_contract
+        jobs
+        m
+        candidates_of
+        (olac_execution olcsac_base);
+  }.
+
+Arguments olcsac_base {CState P candidates_of jobs adm m} _.
+Arguments olcsac_candidates {CState P candidates_of jobs adm m} _.
